progress on stating Oeuf correctness

src/OeufProof.v
@@ -12,8 +12,6 @@ Require Import compcert.common.Events.
 Require Import compcert.common.Globalenvs.
 
 
-Inductive correspond (exp : Untyped.expr) (st : Asm.state).
-
 Inductive simple_star {A : Type} (step : A -> A -> Prop) : A -> A -> Prop :=
 | star_nil :
     forall st,
@@ -24,25 +22,44 @@ Inductive simple_star {A : Type} (step : A -> A -> Prop) : A -> A -> Prop :=
       simple_star step st2 st3 ->
       simple_star step st1 st3.
 
-Theorem OeufUntypedCorrect :
-  forall l md asmprog,
-    transf_untyped_to_asm (l,md) = OK asmprog ->
-    forall expr expr',
-      In expr l ->
-      simple_star Untyped.step expr expr' ->
-      exists rs m rs' m',
-        Asm.initial_state asmprog (Asm.State rs m) /\
-        star Asm.step (Genv.globalenv asmprog) (State rs m) E0 (State rs' m') /\
-        correspond expr' (State rs' m').
+(* Dummy definition, fill in later *)
+Inductive correspond {tys ty} (exp : SourceLang.expr tys ty) (st : Asm.state).
+
+
+Lemma type_dec_eq :
+  forall (t1 t2 : SourceLang.type),
+    { t1 = t2 } + { t1 <> t2 }.
 Proof.
-  induction 3; intros.
-  (* Here we need the "if we have an untyped expr, we get an Asm initial state" lemma *)
-  (* We also need that that initial state corresponds to the expression *)
-  admit.
+  decide equality.
+  destruct t; destruct t0; try decide equality;
+    left; reflexivity.
+Defined.
 
-  (* Here we need the *)
-  admit.
-  
-  (* *)
+
+(* This is crazy *)
+Fixpoint grab_expr {t1s t2s : list SourceLang.type} {ty : SourceLang.type} (exprs : hlist (SourceLang.expr t1s) t2s) (expr : SourceLang.expr t1s ty) : Prop .
+  destruct exprs eqn:?. exact False.
+  destruct (type_dec_eq ty a). exact True.
+  exact (grab_expr _ _ _ h expr).
+Defined.
+
+Inductive initial_state (cu : compilation_unit) : forall tys ty, SourceLang.expr tys ty -> Prop := 
+| initial_intro :
+    forall ty expr,
+      @grab_expr nil (types cu) ty (exprs cu) expr ->
+      initial_state cu nil ty expr.
+    
+      
+Theorem Oeuf_correct :
+  forall cu asmprog,
+    transf_to_asm cu = OK asmprog ->
+    forall tys ty expr,
+      initial_state cu tys ty expr ->
+      forall expr',
+        simple_star SourceLang.step expr expr' ->
+        exists st st',
+          Asm.initial_state asmprog st /\
+          star Asm.step (Genv.globalenv asmprog) st E0 st' /\
+          correspond expr' st'.
+Proof.
 Admitted.
-
